\documentclass{article}
\usepackage{amsmath}
\usepackage{ulem}
\usepackage{cancel}
\newcommand{\mbeq}{\overset{!}{=}}


%Für Berechnungen siehe aufgabe16.py

\begin{document}
 In the task on page 16 we were asked to calculate the theoretical values for the experiment on optical resonators. We were given $R=50mm$ for both plano-convex lenses, $L=45mm$ distance between the lenses. The lenses have a width $b=6.35mm$ and a refraction index $n_{L} = 1.515$ The wavelength of the light will be $\lambda = 632nm$ for the following calculations.\\

 Using the given equation for the waist within the optical resonator

\begin{equation}
\omega_{0}^2 = \frac{\lambda}{\pi}\sqrt{\frac{L}{2}(R-\frac{L}{2})}
\label{omegawithinres}
\end{equation}

we obtain\\

$\omega_{0}^2 = \frac{632nm}{\pi}\sqrt{\frac{4.5mm}{2}(50mm-\frac{4.5mm}{2})} = 4.9*10^(-8) m$\\

The resulting rayleigh length is then\\

$z_{R} = \frac{\pi4.9*10^(-8) m}{632} = 1.2*10^{-8} m$\\
%z_{R} = \frac{\pi*\omega_{0}^2 n}{\lambda} ist schon definiert: \ref{rayleighlength}

%Nützliche Formeln
$D = \frac{n_{L}-1}{R}$

Upon hitting the first mirror, for the light we have
\\\\
$M_{boundary 1}= \begin{pmatrix}
1 & 0\\
D_{12}& 1
\end{pmatrix}$ with $D_{12} = -\frac{n_{mirror 1}-n_{air}}{R}$
\\\\
Then for propagation through the first mirror
\\\\
$M_{propagation 1}= \begin{pmatrix}
1 & \frac{b_1}{n_{mirror 1}}\\
0 & 1
\end{pmatrix}$
\\\\
When leaving the mirror
\\\\
$M_{boundary 2}= \begin{pmatrix}
1 & 0\\
D_{23} & 1
\end{pmatrix}$ with $D_{23} = -\frac{n_{air}-n_{mirror 1}}{R'}$
\\\\
Thus in total we have
$M_{mirror 1}= M_{boundary 1} \cdot M_{propagation 1} \cdot M_{boundary 2} 
\\\\
= \begin{pmatrix}
1 & 0\\
D_{12} & 1
\end{pmatrix} \cdot \begin{pmatrix}
1 & \frac{b_1}{n_{mirror 1}}\\
0 & 1
\end{pmatrix} \cdot \begin{pmatrix}
1 & 0\\
D_{23} & 1
\end{pmatrix}= \begin{pmatrix}
\frac{n_2-b \cdot D_{23}}{n_2} & \frac{b}{n_2}\\
-\frac{-D_{12} \cdot n_2 - D_{23}(-D_{12}b+n_2)}{n_2} & \frac{-D_{12}b+n_2}{n_2}
\end{pmatrix}$
\\\\
Since, $n_{mirror1} = n_{mirror 2} \equiv n_2$ and $D_{12} = \frac{n_{mirror 1}-n_{air}}{R}$ and $R \xrightarrow[]{} \infty$ for the first square boundary, $D_{12} \xrightarrow[]{} 0$

$\Rightarrow{} M_{mirror 1}=\begin{pmatrix}
\frac{n_2-b \cdot D_{23}}{n_2} & \frac{b}{n_2}\\
\frac{D_{23}n_2}{n_2} & 1
\end{pmatrix}$
\\
Applying the same method to the second mirror
\\

$M_{mirror 2}= M_{boundary 3} \cdot M_{propagation 2} \cdot M_{boundary 4}$
\\\\
$M_{mirror 2} = \begin{pmatrix}
1 & 0\\
D_{12}' & 1
\end{pmatrix} \cdot \begin{pmatrix}
1 & \frac{b_1}{n_{mirror 1}}\\
0 & 1
\end{pmatrix} \cdot \begin{pmatrix}
1 & 0\\
0 & 1
\end{pmatrix}=\begin{pmatrix}
1 & \frac{b}{n_2}\\
D'_{12} & \frac{D_{23}b+n_2}{n_2}
\end{pmatrix}$
\\

\end{document}